WIP: writing loop lemmas

nondeterministic_dataflow/Loop.thy
@@ -19,21 +19,11 @@ corec loop_op :: "('op \<rightharpoonup> 'ip) \<Rightarrow> ('ip \<Rightarrow> '
    ) (sound_reads wire buf (choices op)))"
 
 definition feedback_op ( "_ \<up>" [66] 65) where
-  "feedback_op op = map_op projr projr (loop_op (case_sum (Some o Inl) (\<lambda> _. None)) (\<lambda> _. []) op)"
-
-fun assoc where
-  "assoc (Inl x) = Inl (Inl x)"
-| "assoc (Inr (Inl x)) = Inl (Inr x)"
-| "assoc (Inr (Inr x)) = Inr x"
-
-\<comment> \<open>Axiom: A6\<close>
-lemma
-  "(op\<up>)\<up> = (map_op assoc assoc op)\<up>"
-
+  "feedback_op op = map_op projl projl (loop_op (case_sum (\<lambda> _. None) (Some o Inr)) (\<lambda> _. []) op)"
 
 
 end
-
+(* 
 inductive loop_producing :: "('op \<rightharpoonup> 'ip) \<Rightarrow> ('ip \<Rightarrow> 'd buf) \<Rightarrow> ('ip, 'op, 'd) op \<Rightarrow> nat \<Rightarrow> bool" where
   "loop_producing wire buf end_op 0"
 | "p \<notin> ran wire \<Longrightarrow> loop_producing wire buf (Read p f) 0"
@@ -4100,4 +4090,4 @@ end
 
 
                 find_theorems lset while_body_rehistory
-end
+end *)
