nondeterministic_dataflow/Operator.thy
@@ -76,6 +76,35 @@ abbreviation "ARead i f op \<equiv> Choice (cimage (\<lambda> x. if x then op el
 lemma ARead_simp[simp]: "ARead i f op = Choice ({| op, Read i f |})"
   by simp
 
+fun reassoc where
+  "reassoc (Inl (Inl x)) = Inl x"
+| "reassoc (Inl (Inr x)) = Inr (Inl x)"
+| "reassoc (Inr x) = Inr (Inr x)"
+
+fun assoc where
+  "assoc (Inl x) = Inl (Inl x)"
+| "assoc (Inr (Inl x)) = Inl (Inr x)"
+| "assoc (Inr (Inr x)) = Inr x"
+
+lemma reassoc_assoc[simp]:
+  "reassoc o assoc = id"
+  unfolding comp_def
+  apply (rule ext)
+  subgoal for x
+    apply (induct x rule: assoc.induct)
+      apply auto
+    done
+  done
+
+lemma assoc_reassoc[simp]:
+  "assoc o reassoc = id"
+  unfolding comp_def
+  apply (rule ext)
+  subgoal for x
+    apply (induct x rule: reassoc.induct)
+      apply auto
+    done
+  done
 
 type_synonym 'd channel = "'d llist"
 
